Working on the semantics preservation of the symbol table generation phase

x86/Symbtablegenproof.v
@@ -12,20 +12,126 @@ Require Import RelocProgram RelocProgSemantics.
 Import ListNotations.
 Require AsmFacts.
 
-Definition match_prog p tp :=
-  transf_program p = OK tp.
+Open Scope Z_scope.
 
-Lemma transf_program_match:
-  forall p tp, transf_program p = OK tp -> match_prog p tp.
+Ltac monadInvX1 H :=
+  let monadInvX H :=  
+      monadInvX1 H ||
+                 match type of H with
+                 | (?F _ _ _ _ _ _ _ _ = OK _) =>
+                   ((progress simpl in H) || unfold F in H); monadInvX1 H
+                 | (?F _ _ _ _ _ _ _ = OK _) =>
+                   ((progress simpl in H) || unfold F in H); monadInvX1 H
+                 | (?F _ _ _ _ _ _ = OK _) =>
+                   ((progress simpl in H) || unfold F in H); monadInvX1 H
+                 | (?F _ _ _ _ _ = OK _) =>
+                   ((progress simpl in H) || unfold F in H); monadInvX1 H
+                 | (?F _ _ _ _ = OK _) =>
+                   ((progress simpl in H) || unfold F in H); monadInvX1 H
+                 | (?F _ _ _ = OK _) =>
+                   ((progress simpl in H) || unfold F in H); monadInvX1 H
+                 | (?F _ _ = OK _) =>
+                   ((progress simpl in H) || unfold F in H); monadInvX1 H
+                 | (?F _ = OK _) =>
+                   ((progress simpl in H) || unfold F in H); monadInvX1 H
+                 end
+  in
+
+  match type of H with
+  | (OK _ = OK _) =>
+      inversion H; clear H; try subst
+  | (Error _ = OK _) =>
+      discriminate
+  | (bind ?F ?G = OK ?X) =>
+      let x := fresh "x" in (
+      let EQ1 := fresh "EQ" in (
+      let EQ2 := fresh "EQ" in (
+      destruct (bind_inversion F G H) as [x [EQ1 EQ2]];
+      clear H;
+      try (monadInvX EQ1);
+      try (monadInvX1 EQ2))))
+  | (bind2 ?F ?G = OK ?X) =>
+      let x1 := fresh "x" in (
+      let x2 := fresh "x" in (
+      let EQ1 := fresh "EQ" in (
+      let EQ2 := fresh "EQ" in (
+      destruct (bind2_inversion F G H) as [x1 [x2 [EQ1 EQ2]]];
+      clear H;
+      try (monadInvX EQ1);
+      try (monadInvX1 EQ2)))))
+  | (match ?X with left _ => _ | right _ => assertion_failed end = OK _) =>
+      destruct X eqn:?; [try (monadInvX1 H) | discriminate]
+  | (match (negb ?X) with true => _ | false => assertion_failed end = OK _) =>
+      destruct X as [] eqn:?; [discriminate | try (monadInvX1 H)]
+  | (match ?X with true => _ | false => assertion_failed end = OK _) =>
+      destruct X as [] eqn:?; [try (monadInvX1 H) | discriminate]
+  | (mmap ?F ?L = OK ?M) =>
+      generalize (mmap_inversion F L H); intro
+  | (match ?X with Some _ => _ | None => _ end = _) =>
+      let EQ := fresh "EQ" in (
+      destruct X eqn:EQ; try (monadInvX1 H))
+  | (match ?X with pair _ _ => _ end = OK _) =>
+      let EQ := fresh "EQ" in (
+      destruct X eqn:EQ; try (monadInvX1 H))
+  end.
+
+Ltac monadInvX H :=
+  monadInvX1 H ||
+  match type of H with
+  | (?F _ _ _ _ _ _ _ _ = OK _) =>
+      ((progress simpl in H) || unfold F in H); monadInvX1 H
+  | (?F _ _ _ _ _ _ _ = OK _) =>
+      ((progress simpl in H) || unfold F in H); monadInvX1 H
+  | (?F _ _ _ _ _ _ = OK _) =>
+      ((progress simpl in H) || unfold F in H); monadInvX1 H
+  | (?F _ _ _ _ _ = OK _) =>
+      ((progress simpl in H) || unfold F in H); monadInvX1 H
+  | (?F _ _ _ _ = OK _) =>
+      ((progress simpl in H) || unfold F in H); monadInvX1 H
+  | (?F _ _ _ = OK _) =>
+      ((progress simpl in H) || unfold F in H); monadInvX1 H
+  | (?F _ _ = OK _) =>
+      ((progress simpl in H) || unfold F in H); monadInvX1 H
+  | (?F _ = OK _) =>
+      ((progress simpl in H) || unfold F in H); monadInvX1 H
+  end.  
+
+Lemma alignw_le : forall x, x <= align x alignw.
 Proof.
-  intros. subst. red. 
-  auto.
+  intros x. apply align_le. unfold alignw. omega.
+Qed.
+
+
+Lemma divides_align : forall y x,
+    y > 0 -> (y | x) -> align x y = x.
+Proof.
+  intros y x GT DV.
+  unfold align. red in DV. destruct DV as [z DV].
+  subst. replace (z * y + y - 1) with (z * y + (y - 1)) by omega.
+  erewrite Int.Zdiv_shift; eauto.
+  erewrite Z_div_mult; eauto. rewrite Z_mod_mult.
+  rewrite zeq_true. rewrite Z.add_0_r. auto.
+Qed.
+
+Lemma align_idempotent : forall v x,
+    x > 0 -> align (align v x) x = align v x.
+Proof.
+  intros v x H. eapply divides_align; eauto.
+  apply align_divides. auto.
+Qed.
+
+Lemma alignw_divides:
+  forall z,
+    (alignw | align z alignw).
+Proof.
+  intros. apply align_divides. unfold alignw; omega.
 Qed.
 
 
 Section PRESERVATION.
-  Existing Instance inject_perm_all.
+
 Context `{external_calls_prf: ExternalCalls}.
+Existing Instance inject_perm_all.
 
 Local Existing Instance mem_accessors_default.
 
@@ -36,11 +142,204 @@ Variable tprog: program.
 Let ge := Genv.globalenv prog.
 Let tge := globalenv tprog.
 
+Definition match_prog (p: Asm.program) (tp: program) :=
+  transf_program p = OK tp.
+
 Hypothesis TRANSF: match_prog prog tprog.
 
-Lemma transf_program_correct:
-  forall rs, forward_simulation (RealAsm.semantics prog rs) (semantics tprog rs).
+(** ** Definitions for matching  states *)
+
+Definition glob_block_valid (m:mem) := 
+  forall b g, Globalenvs.Genv.find_def ge b = Some g -> Mem.valid_block m b.
+
+Definition regset_inject (j:meminj) (rs rs' : regset) : Prop :=
+  forall r, Val.inject j (rs r) (rs' r).
+
+(** Properties about the memory injection from RealAsm to Relocatable Programs *)   Record match_inj (j: meminj) : Type :=
+  {
+    (** Preservation of finding of instruction *)
+    agree_inj_instrs:
+      forall b b' f ofs ofs' i,
+        Globalenvs.Genv.find_funct_ptr ge b = Some (Internal f) -> 
+        Asm.find_instr (Ptrofs.unsigned ofs) (Asm.fn_code f) = Some i ->
+        j b = Some (b', ofs') -> 
+        Genv.find_instr tge (Vptr b' (Ptrofs.add (Ptrofs.repr ofs') ofs)) = Some i;
+
+    (** Preservation of finding of global symbols *)
+    agree_inj_globs:
+      forall id b,
+        Globalenvs.Genv.find_symbol ge id = Some b ->
+        exists b' ofs', Genv.find_symbol tge id = Some (b', ofs') /\
+                   j b = Some (b', Ptrofs.unsigned ofs');
+
+    (** Preservation of finding of external functions *)
+    agree_inj_ext_funct:
+      forall b f ofs b',
+        Globalenvs.Genv.find_funct_ptr ge b = Some (External f) ->
+        j b = Some (b', ofs) ->
+        Genv.find_ext_funct tge (Vptr b' (Ptrofs.repr ofs)) = Some f;
+
+    (** Preservation of finding of internal functions *)
+    agree_inj_int_funct:
+      forall b f ofs b',
+        Globalenvs.Genv.find_funct_ptr ge b = Some (Internal f) ->
+        j b = Some (b', ofs) ->
+        Genv.find_ext_funct tge (Vptr b' (Ptrofs.repr ofs)) = None;
+  }.
+
+(** Default frame injection *)
+Definition def_frame_inj m := (flat_frameinj (length (Mem.stack m))).
+
+Lemma store_pres_def_frame_inj : forall chunk m1 b ofs v m1',
+    Mem.store chunk m1 b ofs v = Some m1' ->
+    def_frame_inj m1 = def_frame_inj m1'.
+Proof.
+  unfold def_frame_inj. intros.
+  repeat erewrite Mem.push_new_stage_stack. simpl.
+  exploit Mem.store_stack_blocks; eauto. intros. rewrite H0.
+  auto.
+Qed.
+
+Lemma storev_pres_def_frame_inj : forall chunk m1 v1 v2 m1',
+    Mem.storev chunk m1 v1 v2 = Some m1' ->
+    def_frame_inj m1= def_frame_inj m1'.
+Proof.
+  intros until m1'. unfold Mem.storev.
+  destruct v1; try congruence.
+  intros STORE.
+  eapply store_pres_def_frame_inj; eauto.
+Qed.
+
+
+Lemma store_mapped_inject' : 
+  forall (f : meminj) (chunk : memory_chunk) 
+    (m1 : mem) (b1 : block) (ofs : Z) (v1 : val) 
+    (n1 m2 : mem) (b2 : block) (delta : Z) (v2 : val),
+    Mem.inject f (def_frame_inj m1) m1 m2 ->
+    Mem.store chunk m1 b1 ofs v1 = Some n1 ->
+    f b1 = Some (b2, delta) ->
+    Val.inject f v1 v2 ->
+    exists n2 : mem,
+      Mem.store chunk m2 b2 (ofs + delta) v2 = Some n2 /\
+      Mem.inject f (def_frame_inj n1) n1 n2.
+Proof.
+  intros. exploit Mem.store_mapped_inject; eauto. 
+  intros (n2 & STORE & MINJ).
+  eexists. split. eauto.
+  erewrite <- store_pres_def_frame_inj; eauto.
+Qed.
+
+Theorem storev_mapped_inject':
+  forall f chunk m1 a1 v1 n1 m2 a2 v2,
+  Mem.inject f (def_frame_inj m1) m1 m2 ->
+  Mem.storev chunk m1 a1 v1 = Some n1 ->
+  Val.inject f a1 a2 ->
+  Val.inject f v1 v2 ->
+  exists n2,
+    Mem.storev chunk m2 a2 v2 = Some n2 /\ Mem.inject f (def_frame_inj n1) n1 n2.
+Proof.
+  intros. exploit Mem.storev_mapped_inject; eauto. 
+  intros (n2 & STORE & MINJ).
+  eexists. split. eauto.
+  erewrite <- storev_pres_def_frame_inj; eauto.
+Qed.
+
+(** Match States *)
+Inductive match_states: state -> state -> Prop :=
+| match_states_intro: forall (j:meminj) (rs: regset) (m: mem) (rs': regset) (m':mem)
+                        (MINJ: Mem.inject j (def_frame_inj m) m m')
+                        (MATCHINJ: match_inj j)
+                        (RSINJ: regset_inject j rs rs')
+                        (GBVALID: glob_block_valid m),
+    match_states (State rs m) (State rs' m').
+
+
+(** ** Matching of the Initial States *)
+Lemma transf_initial_states : forall rs (SELF: forall j, forall r : PregEq.t, Val.inject j (rs r) (rs r)) st1,
+    RealAsm.initial_state prog rs st1  ->
+    exists st2, initial_state tprog rs st2 /\ match_states st1 st2.
+Proof.
+  Admitted.
+
+
+(** ** Simulation of Single Step Execution *)
+
+(** The internal step preserves the invariant *)
+Lemma exec_instr_step : forall j rs1 rs2 m1 m2 rs1' m1' i id ofs f b
+                        (MINJ: Mem.inject j (def_frame_inj m1) m1 m2)
+                        (MATCHSMINJ: match_inj j)
+                        (RSINJ: regset_inject j rs1 rs2)
+                        (GBVALID: glob_block_valid m1),
+    rs1 PC = Vptr b ofs ->
+    Globalenvs.Genv.find_symbol ge id = Some b ->
+    Globalenvs.Genv.find_funct_ptr ge b = Some (Internal f) ->
+    Asm.find_instr (Ptrofs.unsigned ofs) (Asm.fn_code f) = Some i ->
+    RealAsm.exec_instr ge f i rs1 m1 = Next rs1' m1' ->
+    exists rs2' m2',
+      exec_instr tge i rs2 m2 = Next rs2' m2' /\
+      match_states (State rs1' m1') (State rs2' m2').
 Proof.
 Admitted.
+
+Theorem step_simulation:
+  forall S1 t S2,
+    RealAsm.step ge S1 t S2 ->
+    forall S1' (MS: match_states S1 S1'),
+    exists S2',
+      step tge S1' t S2' /\
+      match_states S2 S2'.
+Proof.
+Admitted.
+
+Lemma transf_final_states:
+  forall st1 st2 r,
+  match_states st1 st2 -> Asm.final_state st1 r -> final_state st2 r.
+Proof.
+  intros st1 st2 r MATCH FINAL.
+  inv FINAL. inv MATCH. constructor. 
+  - red in RSINJ. generalize (RSINJ PC). rewrite H. 
+    unfold Vnullptr. destruct Archi.ptr64; inversion 1; auto.
+  - red in RSINJ. generalize (RSINJ RAX). rewrite H0.
+    inversion 1. auto.
+Qed.
+
+
+Lemma add_external_global_pres_senv :
+  forall e (ge : Genv.t) extfuns,
+  Genv.genv_senv (add_external_global extfuns ge e) = Genv.genv_senv ge.
+Proof.
+  intros. unfold add_external_global.
+  destr.
+Qed.
+
+Lemma add_external_globals_pres_senv :
+  forall stbl (ge : Genv.t) extfuns,
+  Genv.genv_senv (add_external_globals extfuns ge stbl) = Genv.genv_senv ge.
+Proof.
+  induction stbl; intros.
+  - simpl. auto.
+  - simpl. erewrite IHstbl; eauto.
+    rewrite add_external_global_pres_senv. auto.
+Qed.
+
+
+Lemma transf_program_correct:
+  forward_simulation (RealAsm.semantics prog (Pregmap.init Vundef)) 
+                     (semantics tprog (Pregmap.init Vundef)).
+Proof.
+  intros. apply forward_simulation_step with match_states.
+  - simpl. intros. 
+    unfold match_prog in TRANSF. unfold transf_program in TRANSF.
+    repeat destr_in TRANSF. cbn.
+    rewrite add_external_globals_pres_senv. cbn. auto.
+  - simpl. intros s1 IS. 
+    exploit transf_initial_states; eauto.
+    intros.
+    rewrite Pregmap.gi. auto.
+  - simpl. intros s1 s2 r MS FS. eapply transf_final_states; eauto.
+  - simpl. intros s1 t s1' STEP s2 MS. 
+    edestruct step_simulation as (STEP' & MS'); eauto.
+Qed.
+
 
 End PRESERVATION.
